feat: unified model for specifying expected chip properties

SP1Chips/AddChip.lean
@@ -1,23 +1,34 @@
-import SP1Foundations
-import SP1Operations
+import SP1Chips.SP1Chip
 
-structure AddChip where
-  state : CPUState
-  adapter : RTypeReader U16
-  add_operation : AddOperation
-  is_real : U1
+def AddChip (state : CPUState) (adapter : RTypeReader U16)
+    (add_operation : AddOperation) (is_real : U1) : SP1Chip where
+  -- NOTE: Currently missing all air interactions
+  constraint_set := {
+    .assertZero (is_real * (is_real - 1)),
+    .assertZero (is_real * (is_real - 1)),
+    .assertZero (is_real * (((((adapter.op_b_memory.prev_value[0] + adapter.op_c_memory.prev_value[0]) - add_operation.value[0]) + 0) * 2013235201) * (((((adapter.op_b_memory.prev_value[0] + adapter.op_c_memory.prev_value[0]) - add_operation.value[0]) + 0) * 2013235201) - 1))),
+    .assertZero (is_real * (((((adapter.op_b_memory.prev_value[1] + adapter.op_c_memory.prev_value[1]) - add_operation.value[1]) + ((((adapter.op_b_memory.prev_value[0] + adapter.op_c_memory.prev_value[0]) - add_operation.value[0]) + 0) * 2013235201)) * 2013235201) * (((((adapter.op_b_memory.prev_value[1] + adapter.op_c_memory.prev_value[1]) - add_operation.value[1]) + ((((adapter.op_b_memory.prev_value[0] + adapter.op_c_memory.prev_value[0]) - add_operation.value[0]) + 0) * 2013235201)) * 2013235201) - 1))),
+    .assertZero (is_real * (is_real - 1)),
+    .assertZero (is_real * (is_real - 1)),
+    .assertZero (adapter.op_a_0 * (add_operation.value[0] - 0)),
+    .assertZero (adapter.op_a_0 * (add_operation.value[1] - 0)),
+    .assertZero (is_real * (is_real - 1)),
+    .assertZero (is_real * (is_real - 1)),
+    .assertZero (is_real * (is_real - 1))
+  }
+  constraint_prop := sorry
+  compute_spec := add_operation.spec adapter.b adapter.c is_real
+  flow_spec := state.spec (state.pc + 4) 4 is_real
+  memory_spec := adapter.spec state.shard state.clk state.pc 0 /- Opcode::ADD -/ add_operation.value is_real
 
-namespace AddChip
-
--- What we expect the generated constraint to look like:
-def constraints
-  (chip : AddChip) : Prop :=
-  let ⟨state, adapter, add_operation, is_real⟩ := chip
-  state.spec (state.pc + 4) 4 is_real
-  ∧ add_operation.spec adapter.b adapter.c is_real
-  ∧ adapter.spec state.shard state.clk state.pc 0 /- Opcode::ADD -/ add_operation.value is_real
-
-end AddChip
+/-- The constraints on add chip imply the constraints of the underlying add operation. -/
+lemma AddChip.constraintSet_imp_addOperation_constratins
+    (state : CPUState) (adapter : RTypeReader U16)
+    (add_operation : AddOperation) (is_real : U1) :
+    add_operation.constraints adapter.op_b_memory.prev_value adapter.op_c_memory.prev_value is_real ⊆
+      (AddChip state adapter add_operation is_real).constraint_set := by
+  simp [AddChip, AddOperation.constraints, Finset.insert_subset_iff, Finset.singleton_subset_iff]
+  sorry
 
 /-
 
