SP1Chips.lean
@@ -1,1 +1,2 @@
 import SP1Chips.AddChip
+import SP1Chips.SP1Chip
