SP1Chips/SP1Chip.lean
@@ -1,0 +1,34 @@
+import SP1Foundations
+import SP1Operations
+
+structure SP1Chip where
+  /-- Set of constraints extracted from source code. -/
+  constraint_set : Finset SP1Constraint
+  /-- Proposition corresponding to constraints, see `constraints_sound` for correctness. -/
+  constraint_prop : Prop
+  /-- The expected computational behavior of the chip. -/
+  compute_spec : Prop
+  /-- The expected control flow effect of the chip. -/
+  flow_spec : Prop
+  /-- The expected memory effects of the chip. -/
+  memory_spec : Prop
+
+namespace SP1Chip
+
+/-- TODO: Should this be an `iff`? Or should we allow the constraint set to be stronger than the prop? -/
+def constraints_sound (chip : SP1Chip) : Prop :=
+  constraintSet_toProp chip.constraint_set ↔ chip.constraint_prop
+
+/-- Constraints are enough to imply computation is correct -/
+def compute_correct (chip : SP1Chip) : Prop :=
+  chip.constraint_prop → chip.compute_spec
+
+/-- Constraints are enough to imply control flow is correct -/
+def flow_correct (chip : SP1Chip) : Prop :=
+  chip.constraint_prop → chip.flow_spec
+
+/-- Constraints are enough to imply memort is correct -/
+def memory_correct (chip : SP1Chip) : Prop :=
+  chip.constraint_prop → chip.memory_spec
+
+end SP1Chip
